cp:   1) changed 'val', 'memval' and 'memory_chunk' to be integers with arbitrary size. Memory stores the bitsize of data stored. The bitsize to load must match its stored bitsize, otherwise, the behavior is undefined, because LLVM allows underlying HWs to optimize the unused bits arbitrarily. Some properties in Memdata.v are broken.   2) more lemmas for Z.
git-svn-id: https://webdav.seas.upenn.edu/svn/sol/vol@2680 eef5ea85-cc2e-0410-bd84-0fae1f012da8

src/ssa/compcert/Memdata.v
@@ -22,19 +22,157 @@ Require Import Integers.
 Require Import Floats.
 Require Import Values.
 
+Lemma Z_of_S_gt_O : forall n, Z_of_nat (S n) > 0.
+Proof.
+  intros.
+  assert (J:=@O_lt_Z_of_S n).
+  auto with zarith.
+Qed.
+
+
+Definition ZRdiv (a b:Z) : Z :=
+  if zeq (a mod b) 0
+  then a / b
+  else a / b + 1.
+
+Lemma ZRdiv_prop1 : forall a b, b >0 -> b * (ZRdiv a b) >= a.
+Proof.
+  intros. unfold ZRdiv.
+  destruct (zeq (a mod b) 0).
+    rewrite <- Z_div_exact_full_2; auto with zarith.
+    
+    rewrite Zmult_plus_distr_r.
+    rewrite (Zmult_comm b 1) .
+    rewrite Zmult_1_l.
+    assert (J:=@Z_mod_lt a b H).
+    assert (J':=@Z_div_mod_eq_full a b). 
+    auto with zarith.
+Qed.
+
+Lemma ZRdiv_prop2 : forall a b, a >=0 -> b > 0 -> ZRdiv a b >= 0.
+Proof.
+  intros.
+  unfold ZRdiv.
+  destruct (zeq (a mod b) 0).
+    apply Z_div_ge0; auto.
+    assert (J:=@Z_div_ge0 a b H0 H). auto with zarith.
+Qed.
+
+Lemma Z_div_gt0 : forall a b,
+  a > 0 -> b > 0 -> a / b > 0.
+Proof.
+  intros.
+  auto with zarith.
+Admitted.
+
+Lemma ZRdiv_prop3 : forall a b, a > 0 -> b > 0 -> ZRdiv a b > 0.
+Proof.
+  intros.
+  unfold ZRdiv.
+  destruct (zeq (a mod b) 0).
+    apply Z_div_gt0; auto.
+    assert (J:=@Z_div_gt0 a b H H0). auto with zarith.
+Qed.
+
+Lemma ZRdiv_prop4 : forall wz,
+  ZRdiv (Z_of_nat (S wz)) 8 >= 0.
+Proof.
+  intro.
+  apply ZRdiv_prop2; try solve [auto with zarith | apply Z_of_S_gt_O].
+Qed.
+
+Lemma mod_prop1 : forall wz,
+  Z_of_nat (S wz) mod 8 >= 0.
+Proof.
+  intro wz.
+  destruct (Z_mod_lt (Z_of_nat (S wz)) 8);
+    auto with zarith.
+Qed.    
+
+Lemma nat_of_Z_pos:
+  forall n, n > 0 -> (nat_of_Z n > O)%nat.
+Proof.
+  intros.
+  destruct n; unfold Zle; simpl; try omega.
+Admitted.
+
+Lemma nat_of_Z_inj : forall z1 z2,
+  z1 >= 0 ->
+  z2 >= 0 ->
+  nat_of_Z z1 = nat_of_Z z2 ->
+  z1 = z2.
+Admitted.
+
+Lemma zdiv_zmod_prop1 : forall a1 a2 b,
+  b <> 0 ->
+  a1 / b = a2 / b ->
+  a1 mod b = a2 mod b ->
+  a1 = a2.
+Proof.
+  intros.
+  rewrite (@Z_div_mod_eq_full a1 b H).
+  rewrite (@Z_div_mod_eq_full a2 b H).
+  rewrite H0. rewrite H1.
+  auto.
+Qed.
+
+Lemma zrdiv_zmod_prop1 : forall a1 a2 b,
+  b <> 0 ->
+  ZRdiv a1 b = ZRdiv a2 b ->
+  a1 mod b = a2 mod b ->
+  a1 = a2.
+Proof.
+  intros.
+  unfold ZRdiv in H0.
+  rewrite H1 in H0.
+  destruct (zeq (a2 mod b) 0).
+    eapply zdiv_zmod_prop1; eauto.
+    apply zdiv_zmod_prop1 with (b:=b); auto.
+      eauto with zarith.
+Qed.
+
 (** * Properties of memory chunks *)
 
 (** Memory reads and writes are performed by quantities called memory chunks,
   encoding the type, size and signedness of the chunk being addressed.
   The following functions extract the size information from a chunk. *)
 
+Definition bytesize_chunk (wz:nat) := ZRdiv (Z_of_nat (S wz)) 8.
+Definition bytesize_chunk_nat (wz:nat) := nat_of_Z (bytesize_chunk wz).
+Definition wordsize_chunk (wz:nat) := (bytesize_chunk wz) * 8.
+
+Lemma bytesize_chunk_pos:
+  forall wz, bytesize_chunk wz > 0.
+Proof.
+  intros. unfold bytesize_chunk.
+  apply ZRdiv_prop3; auto with zarith.
+    assert (J:=@O_lt_Z_of_S wz).
+    auto with zarith.
+Qed.
+
+Lemma bytesize_chunk_conv:
+  forall wz, bytesize_chunk wz = Z_of_nat (bytesize_chunk_nat wz).
+Proof.
+  intros.
+  unfold bytesize_chunk, bytesize_chunk_nat, bytesize_chunk.
+  decEq. 
+  rewrite nat_of_Z_eq. auto.
+    apply ZRdiv_prop2; auto with zarith.
+Qed.
+
+Lemma bytesize_chunk_nat_pos:
+  forall wz, exists n, bytesize_chunk_nat wz = S n.
+Proof.
+  intros. 
+  generalize (bytesize_chunk_pos wz). rewrite bytesize_chunk_conv. 
+  destruct (bytesize_chunk_nat wz).
+  simpl; intros; omegaContradiction.
+  intros; exists n; auto.
+Qed.
+
 Definition size_chunk (chunk: memory_chunk) : Z :=
   match chunk with
-  | Mint8signed => 1
-  | Mint8unsigned => 1
-  | Mint16signed => 2
-  | Mint16unsigned => 2
-  | Mint32 => 4
+  | Mint wz => bytesize_chunk wz
   | Mfloat32 => 4
   | Mfloat64 => 8
   end.
@@ -42,7 +180,7 @@ Definition size_chunk (chunk: memory_chunk) : Z :=
 Lemma size_chunk_pos:
   forall chunk, size_chunk chunk > 0.
 Proof.
-  intros. destruct chunk; simpl; omega.
+  intros. destruct chunk; simpl; try solve [omega | apply bytesize_chunk_pos].
 Qed.
 
 Definition size_chunk_nat (chunk: memory_chunk) : nat :=
@@ -51,7 +189,7 @@ Definition size_chunk_nat (chunk: memory_chunk) : nat :=
 Lemma size_chunk_conv:
   forall chunk, size_chunk chunk = Z_of_nat (size_chunk_nat chunk).
 Proof.
-  intros. destruct chunk; reflexivity.
+  intros. destruct chunk; try solve [reflexivity | apply bytesize_chunk_conv].
 Qed.
 
 Lemma size_chunk_nat_pos:
@@ -62,6 +200,14 @@ Proof.
   destruct (size_chunk_nat chunk).
   simpl; intros; omegaContradiction.
   intros; exists n; auto.
+Qed.
+
+Lemma size_chunk_nat_pos':
+  forall chunk, (size_chunk_nat chunk > 0)%nat.
+Proof.
+  intros.
+  destruct (@size_chunk_nat_pos chunk) as [n J].
+  rewrite J. omega.
 Qed.
 
 (** Memory reads and writes must respect alignment constraints:
@@ -76,10 +222,7 @@ Qed.
 
 Definition align_chunk (chunk: memory_chunk) : Z := 
   match chunk with
-  | Mint8signed => 1
-  | Mint8unsigned => 1
-  | Mint16signed => 2
-  | Mint16unsigned => 2
+  | Mint wz => 1
   | _ => 4
   end.
 
@@ -92,16 +235,21 @@ Qed.
 Lemma align_size_chunk_divides:
   forall chunk, (align_chunk chunk | size_chunk chunk).
 Proof.
-  intros. destruct chunk; simpl; try apply Zdivide_refl. exists 2; auto. 
+  intros. destruct chunk; simpl; try solve [
+    apply Zdivide_refl |
+    destruct (le_lt_dec n 1); auto with zarith |
+    exists 2; auto ]. 
 Qed.
 
+(* Broken
 Lemma align_chunk_compat:
   forall chunk1 chunk2,
   size_chunk chunk1 = size_chunk chunk2 -> align_chunk chunk1 = align_chunk chunk2.
 Proof.
   intros chunk1 chunk2. 
-  destruct chunk1; destruct chunk2; simpl; congruence.
+  destruct chunk1; destruct chunk2; simpl; try congruence.
 Qed.
+*)
 
 (** * Memory values *)
 
@@ -116,7 +264,7 @@ Qed.
 
 Inductive memval: Type :=
   | Undef: memval
-  | Byte: byte -> memval
+  | Byte: nat -> byte -> memval
   | Pointer: block -> int32 -> nat -> memval.
 
 (** * Encoding and decoding integers *)
@@ -124,46 +272,18 @@ Inductive memval: Type :=
 (** We define functions to convert between integers and lists of bytes
   according to a given memory chunk. *)
 
+(** bytes_of_int *)
+
 Fixpoint bytes_of_int (n: nat) (x: Z) {struct n}: list byte :=
   match n with
   | O => nil
   | S m => Int.repr 7 x :: bytes_of_int m (x / 256)
   end.
 
-Fixpoint int_of_bytes (l: list byte): Z :=
-  match l with
-  | nil => 0
-  | b :: l' => Int.unsigned 7 b + int_of_bytes l' * 256
-  end.
-
 Lemma length_bytes_of_int:
   forall n x, length (bytes_of_int n x) = n.
 Proof.
   induction n; simpl; intros. auto. decEq. auto.
-Qed.
-
-Lemma int_of_bytes_of_int:
-  forall n x,
-  int_of_bytes (bytes_of_int n x) = x mod (two_p (Z_of_nat n * 8)).
-Proof.
-  induction n; intros.
-  simpl. rewrite Zmod_1_r. auto.
-  rewrite inj_S. simpl.
-  replace (Zsucc (Z_of_nat n) * 8) with (Z_of_nat n * 8 + 8) by omega.
-  rewrite two_p_is_exp; try omega. 
-  rewrite Zmod_recombine. rewrite IHn. rewrite Zplus_comm. reflexivity. 
-  apply two_p_gt_ZERO. omega. apply two_p_gt_ZERO. omega.
-Qed.
-
-Lemma int_of_bytes_of_int_2:
-  forall n x,
-  (n = 1 \/ n = 2)%nat ->
-  Int.repr 31 (int_of_bytes (bytes_of_int n (Int.unsigned 31 x))) = Int.zero_ext 31 (Z_of_nat n * 8) x.
-Proof.
-  intros. rewrite int_of_bytes_of_int. 
-  rewrite <- (Int.repr_unsigned 31 (Int.zero_ext 31 (Z_of_nat n * 8) x)). 
-  decEq. symmetry. apply Int.zero_ext_mod.
-  destruct H; subst n; compute; auto.
 Qed.
 
 Lemma bytes_of_int_mod:
@@ -186,13 +306,263 @@ Proof.
   rewrite <- Z_div_plus_full_l. decEq. change (two_p 8) with 256. ring. omega.
 Qed.
 
+Lemma bytes_of_int_mod':
+  forall z x y,
+  z >= 0 ->
+  Int.eqmod (two_p (z * 8)) x y ->
+  bytes_of_int (nat_of_Z z) x =
+  bytes_of_int (nat_of_Z z) y.
+Proof.
+  intros.
+  rewrite <- (@nat_of_Z_eq z) in H0; auto.
+  apply bytes_of_int_mod; auto.
+Qed.
+
+Lemma bytes_of_int_prop1: forall n z,
+  (n > 0)%nat ->
+  exists b, exists bl, 
+    bytes_of_int n z = b::bl.
+Proof. Admitted.
+
+(** int_of_bytes *)
+
+Fixpoint int_of_bytes (l: list byte): Z :=
+  match l with
+  | nil => 0
+  | b :: l' => Int.unsigned 7 b + int_of_bytes l' * 256
+  end.
+
+Lemma int_of_bytes_of_int:
+  forall n x,
+  int_of_bytes (bytes_of_int n x) = x mod (two_p (Z_of_nat n * 8)).
+Proof.
+  induction n; intros.
+  simpl. rewrite Zmod_1_r. auto.
+  rewrite inj_S. simpl.
+  replace (Zsucc (Z_of_nat n) * 8) with (Z_of_nat n * 8 + 8) by omega.
+  rewrite two_p_is_exp; try omega. 
+  rewrite Zmod_recombine. rewrite IHn. rewrite Zplus_comm. reflexivity. 
+  apply two_p_gt_ZERO. omega. apply two_p_gt_ZERO. omega.
+Qed.
+
+Lemma int_of_bytes_of_int_wz:
+  forall n wz x,
+  0 < Z_of_nat n ->
+  Int.repr wz (int_of_bytes (bytes_of_int n (Int.unsigned wz x))) = 
+  Int.zero_ext wz (Z_of_nat n * 8) x.
+Proof.
+  intros. rewrite int_of_bytes_of_int. 
+  rewrite <- (Int.repr_unsigned wz (Int.zero_ext wz (Z_of_nat n * 8) x)). 
+  decEq. symmetry. apply Int.zero_ext_mod; try solve [omega]. 
+Qed.
+
+Lemma int_of_bytes_of_int_2:
+  forall n x,
+  (n = 1 \/ n = 2)%nat ->
+  Int.repr 31 (int_of_bytes (bytes_of_int n (Int.unsigned 31 x))) = Int.zero_ext 31 (Z_of_nat n * 8) x.
+Proof.
+  intros. apply int_of_bytes_of_int_wz.
+  destruct H; subst n; compute; auto.
+Qed.
+
+Definition inj_bytes (bl: list byte) : list memval :=
+  List.map (Byte 8) bl.
+
+Remark length_inj_bytes:
+  forall bl, length (inj_bytes bl) = length bl.
+Proof.
+  intros. apply List.map_length. 
+Qed.
+
+(** inj_int *)
+
+Definition inj_int (wz:nat) (x: Int.int wz) : list memval :=
+  let z := Int.unsigned wz x in
+  let n := Z_of_nat (S wz) in
+  let m := n mod 8 in
+  let sz := ZRdiv n 8 in
+  let bl := bytes_of_int (nat_of_Z sz) z in
+  match bl with
+  | nil => nil
+  | b::bl' => Byte (nat_of_Z m) b :: inj_bytes bl'
+  end.
+
+Lemma length_inj_int : forall wz n,
+  length (inj_int wz n) = bytesize_chunk_nat wz.
+Proof.
+  intros.
+  unfold inj_int, bytesize_chunk_nat, bytesize_chunk.
+  assert (J:=@length_bytes_of_int 
+    (nat_of_Z (ZRdiv (Z_of_nat (S wz)) 8)) 
+    (Int.unsigned wz n)).
+  remember (bytes_of_int (nat_of_Z (ZRdiv (Z_of_nat (S wz)) 8)) 
+    (Int.unsigned wz n)) as bl.
+  destruct bl; auto.
+    simpl in *.
+    rewrite <- J.
+    decEq.
+    apply map_length.
+Qed.   
+
+(** proj_bytes *)
+
+Fixpoint proj_bytes (n:nat) (vl: list memval) {struct n} : option (list byte) :=
+  match n, vl with
+  | O, nil => Some nil
+  | S m, Byte wz b :: vl' =>
+      if eq_nat_dec wz 8 
+      then
+        match (proj_bytes m vl') with
+        | Some bl' => Some (b :: bl')
+        | None => None
+        end
+      else None
+  | _, _ => None
+  end.
+
+Remark proj_inj_bytes:
+  forall bl, proj_bytes (length bl) (inj_bytes bl) = Some bl.
+Proof.
+  induction bl; simpl. auto. rewrite IHbl. auto.
+Qed.
+
+Lemma inj_proj_bytes:
+  forall cl bl, proj_bytes (length cl) cl = Some bl -> cl = inj_bytes bl.
+Proof.
+  induction cl; simpl; intros. 
+  inv H; auto.
+  destruct a; try congruence.
+  destruct (eq_nat_dec n 8); subst.
+    destruct (proj_bytes (length cl) cl); inv H.
+      simpl. decEq. auto.
+      inversion H.
+Qed.
+
+Lemma proj_bytes_prop1 : forall n wz x bl,
+  proj_bytes n (map (Byte 8) (bytes_of_int n (Int.unsigned wz x / 256))) = Some bl ->
+  x = Int.repr wz (Int.unsigned wz x mod Int.modulus 7 + int_of_bytes bl * 256).
+Admitted.
+
+Lemma proj_bytes_prop2: forall vl n,
+  length vl = n ->
+  exists bl, proj_bytes n (map (Byte 8) vl) = Some bl.
+Proof.
+  induction vl; intros; subst; simpl.
+    exists nil. auto.
+    
+    destruct (@IHvl (length vl)) as [bl J]; auto.
+    rewrite J.
+    exists (a::bl). auto.
+Qed.
+
+Lemma proj_bytes_prop3: forall vl n bl,
+  proj_bytes n (map (Byte 8) vl) = Some bl ->
+  length bl = n /\ length vl = n.
+Admitted.
+
+(** proj_int *)
+
+Definition proj_int (wz:nat) (vl: list memval) : option (Int.int wz) :=
+  let n := Z_of_nat (S wz) in
+  let m := nat_of_Z (n mod 8) in
+  let sz := nat_of_Z (ZRdiv n 8) in
+  match sz, vl with
+  | O, nil => None
+  | S n', Byte wz0 b :: vl' =>
+    if eq_nat_dec wz0 m
+    then 
+      match (proj_bytes n' vl') with
+      | Some bl' => Some (Int.repr wz (int_of_bytes (b::bl')))
+      | None => None
+      end
+    else None
+  | _, _ => None
+  end.
+
+Lemma proj_inj_int_eq : 
+  forall wz x,
+  proj_int wz (inj_int wz x) = Some x.
+Proof.
+  intros.
+  unfold proj_int, inj_int.
+  remember (nat_of_Z (ZRdiv (Z_of_nat (S wz)) 8)) as n.
+  assert (n > 0)%nat.
+    subst.
+    apply nat_of_Z_pos.
+    apply ZRdiv_prop3; auto with zarith.
+      apply Z_of_S_gt_O.
+  Opaque Z_of_nat.
+  destruct n; simpl.
+    contradict H; omega.
+
+    destruct (eq_nat_dec 
+      (nat_of_Z ((Z_of_nat (S wz)) mod 8))
+      (nat_of_Z ((Z_of_nat (S wz)) mod 8))
+      ).
+      destruct (@proj_bytes_prop2 (bytes_of_int n (Int.unsigned wz x/256)) n) 
+        as [bl EQ].
+        apply length_bytes_of_int.
+        unfold inj_bytes.
+        rewrite EQ. 
+
+        apply proj_bytes_prop1 in EQ. rewrite <- EQ. auto.
+      contradict n0; auto.
+Qed.
+
+Lemma proj_inj_int_neq : 
+  forall wz1 wz2 x,
+  wz1 <> wz2 ->
+  proj_int wz1 (inj_int wz2 x) = None.
+Proof.
+  intros.
+  unfold proj_int, inj_int.
+  remember (nat_of_Z (ZRdiv (Z_of_nat (S wz1)) 8)) as n.
+  assert (n > 0)%nat.
+    subst.
+    apply nat_of_Z_pos.
+    apply ZRdiv_prop3; auto with zarith.
+      apply Z_of_S_gt_O.
+  Opaque Z_of_nat.
+  destruct n; simpl.
+    contradict H; omega.
+    destruct (@bytes_of_int_prop1 
+      (nat_of_Z (ZRdiv (Z_of_nat (S wz2)) 8))
+      (Int.unsigned wz2 x))
+      as [b [bl EQ]].
+      apply nat_of_Z_pos.
+      apply ZRdiv_prop3; auto with zarith.
+        apply Z_of_S_gt_O.
+    rewrite EQ.      
+
+    unfold inj_bytes.
+    destruct (eq_nat_dec 
+      (nat_of_Z ((Z_of_nat (S wz2)) mod 8))
+      (nat_of_Z ((Z_of_nat (S wz1)) mod 8))
+      ); auto.
+      apply nat_of_Z_inj in e; try solve [apply mod_prop1].
+        remember (proj_bytes n (map (Byte 8) bl)) as R.
+        destruct R; auto.
+          symmetry in HeqR.
+          apply proj_bytes_prop3 in HeqR.
+          destruct HeqR as [EQ1 EQ2]; subst.
+          assert(J:=@length_bytes_of_int (nat_of_Z (ZRdiv (Z_of_nat (S wz2)) 8)) (Int.unsigned wz2 x)).
+          rewrite EQ in J.
+          simpl in J. rewrite EQ2 in J.
+          rewrite Heqn in J.
+          apply nat_of_Z_inj in J; try solve [apply ZRdiv_prop4].
+            apply zrdiv_zmod_prop1 in J; auto with zarith.
+              apply inj_eq_rev in J; auto.
+              inversion J; subst.        
+              contradict H; auto.
+Qed.
+
 Parameter big_endian: bool.
 
-Definition rev_if_be (l: list byte) : list byte :=
+Definition rev_if_be (A:Type) (l: list A) : list A :=
   if big_endian then List.rev l else l.
 
 Lemma rev_if_be_involutive:
-  forall l, rev_if_be (rev_if_be l) = l.
+  forall A l, rev_if_be A (rev_if_be A l) = l.
 Proof.
   intros; unfold rev_if_be; destruct big_endian. 
   apply List.rev_involutive. 
@@ -200,190 +570,76 @@ Proof.
 Qed.
 
 Lemma rev_if_be_length:
-  forall l, length (rev_if_be l) = length l.
+  forall A l, length (rev_if_be A l) = length l.
 Proof.
   intros; unfold rev_if_be; destruct big_endian.
   apply List.rev_length.
   auto.
 Qed.
 
-Definition encode_int (c: memory_chunk) (x: int32) : list byte :=
-  let n := Int.unsigned 31 x in
-  rev_if_be (match c with
-  | Mint8signed | Mint8unsigned => bytes_of_int 1%nat n
-  | Mint16signed | Mint16unsigned => bytes_of_int 2%nat n
-  | Mint32 => bytes_of_int 4%nat n
-  | Mfloat32 => bytes_of_int 4%nat 0
-  | Mfloat64 => bytes_of_int 8%nat 0
-  end).
+(* generate the stored bytes of x (with size wz). *)
+Definition encode_int (wz:nat) (x: Int.int wz) : list memval :=
+  rev_if_be _ (inj_int wz x).
 
-Definition decode_int (c: memory_chunk) (b: list byte) : int32 :=
-  let b' := rev_if_be b in
-  match c with
-  | Mint8signed => Int.sign_ext 31 8 (Int.repr 31 (int_of_bytes b'))
-  | Mint8unsigned => Int.zero_ext 31 8 (Int.repr 31 (int_of_bytes b'))
-  | Mint16signed => Int.sign_ext 31 16 (Int.repr 31 (int_of_bytes b'))
-  | Mint16unsigned => Int.zero_ext 31 16 (Int.repr 31 (int_of_bytes b'))
-  | Mint32 => Int.repr 31 (int_of_bytes b')
-  | Mfloat32 => Int.zero 31 
-  | Mfloat64 => Int.zero 31
+Definition decode_int (b: list memval) (wz:nat) : val :=
+  let b' := rev_if_be _ b in
+  match (proj_int wz b') with
+  | Some i => Vint wz i
+  | None => Vundef
   end.
 
 Lemma encode_int_length:
-  forall chunk n, length(encode_int chunk n) = size_chunk_nat chunk.
+  forall wz n, length(encode_int wz n) = bytesize_chunk_nat wz.
 Proof.
   intros. unfold encode_int. rewrite rev_if_be_length.
-  destruct chunk; rewrite length_bytes_of_int; reflexivity.
+  apply length_inj_int.
 Qed.
 
-Lemma decode_encode_int:
-  forall c x,
-  decode_int c (encode_int c x) =
-  match c with
-  | Mint8signed => Int.sign_ext 31 8 x
-  | Mint8unsigned => Int.zero_ext 31 8 x
-  | Mint16signed => Int.sign_ext 31 16 x
-  | Mint16unsigned => Int.zero_ext 31 16 x
-  | Mint32 => x
-  | Mfloat32 => Int.zero 31
-  | Mfloat64 => Int.zero 31
-  end.
+Lemma decode_encode_int_eq:
+  forall wz x,
+  decode_int (encode_int wz x) wz = Vint wz x.
 Proof.
-  intros. unfold decode_int, encode_int; destruct c; auto;
+  intros. unfold decode_int, encode_int; auto;
   rewrite rev_if_be_involutive.
-  rewrite int_of_bytes_of_int_2; auto.
-  apply Int.sign_ext_zero_ext. compute; auto.
-  rewrite int_of_bytes_of_int_2; auto.
-  apply Int.zero_ext_idem. compute; auto.
-  rewrite int_of_bytes_of_int_2; auto.
-  apply Int.sign_ext_zero_ext. compute; auto.
-  rewrite int_of_bytes_of_int_2; auto.
-  apply Int.zero_ext_idem. compute; auto.
-  rewrite int_of_bytes_of_int. 
-  transitivity (Int.repr 31 (Int.unsigned 31 x)). 
-  apply Int.eqm_samerepr. apply Int.eqm_sym. apply Int.eqmod_mod. apply two_p_gt_ZERO. omega. 
-  apply Int.repr_unsigned.
+
+  rewrite proj_inj_int_eq. auto.
 Qed.
 
-Lemma encode_int8_signed_unsigned: forall n,
-  encode_int Mint8signed n = encode_int Mint8unsigned n.
+Lemma decode_encode_int_neq:
+  forall wz1 wz2 x,
+  wz1 <> wz2 ->
+  decode_int (encode_int wz1 x) wz2 = Vundef.
 Proof.
-  intros; reflexivity.
+  intros. unfold decode_int, encode_int; auto;
+  rewrite rev_if_be_involutive.
+
+  rewrite proj_inj_int_neq; auto.
 Qed.
 
-Remark encode_8_mod:
-  forall x y,
-  Int.eqmod (two_p 8) (Int.unsigned 31 x) (Int.unsigned 31 y) ->
-  encode_int Mint8unsigned x = encode_int Mint8unsigned y.
+Remark encode_mod:
+  forall wz x y, 
+  Int.eqmod (two_p (wordsize_chunk wz)) (Int.unsigned wz x) (Int.unsigned wz y) ->
+  encode_int wz x = encode_int wz y.
 Proof.
-  intros. unfold encode_int. decEq. apply bytes_of_int_mod. auto.
-Qed.
-
-Lemma encode_int8_zero_ext:
-  forall x,
-  encode_int Mint8unsigned (Int.zero_ext 31 8 x) = encode_int Mint8unsigned x.
-Proof.
-  intros. apply encode_8_mod. apply Int.eqmod_zero_ext. compute; auto.
-Qed.
-
-Lemma encode_int8_sign_ext:
-  forall x,
-  encode_int Mint8signed (Int.sign_ext 31 8 x) = encode_int Mint8signed x.
-Proof.
-  intros. repeat rewrite encode_int8_signed_unsigned. 
-  apply encode_8_mod. eapply Int.eqmod_trans.
-  apply (Int.eqm_eqmod_two_p 31). compute; auto. 
-  apply Int.eqm_sym. apply Int.eqm_signed_unsigned.
-  apply Int.eqmod_sign_ext. compute; auto.
-Qed.
-
-Lemma encode_int16_signed_unsigned: forall n,
-  encode_int Mint16signed n = encode_int Mint16unsigned n.
-Proof.
-  intros; reflexivity.
-Qed.
-
-Remark encode_16_mod:
-  forall x y,
-  Int.eqmod (two_p 16) (Int.unsigned 31 x) (Int.unsigned 31 y) ->
-  encode_int Mint16unsigned x = encode_int Mint16unsigned y.
-Proof.
-  intros. unfold encode_int. decEq. apply bytes_of_int_mod. auto.
-Qed.
-
-Lemma encode_int16_zero_ext:
-  forall x,
-  encode_int Mint16unsigned (Int.zero_ext 31 16 x) = encode_int Mint16unsigned x.
-Proof.
-  intros. apply encode_16_mod. apply Int.eqmod_zero_ext. compute; auto.
-Qed.
-
-Lemma encode_int16_sign_ext:
-  forall x,
-  encode_int Mint16signed (Int.sign_ext 31 16 x) = encode_int Mint16signed x.
-Proof.
-  intros. repeat rewrite encode_int16_signed_unsigned. 
-  apply encode_16_mod. eapply Int.eqmod_trans.
-  apply (Int.eqm_eqmod_two_p 31). compute; auto. 
-  apply Int.eqm_sym. apply Int.eqm_signed_unsigned.
-  apply Int.eqmod_sign_ext. compute; auto.
-Qed.
-
-Lemma decode_int8_zero_ext:
-  forall l,
-  Int.zero_ext 31 8 (decode_int Mint8unsigned l) = decode_int Mint8unsigned l.
-Proof.
-  intros; simpl. apply Int.zero_ext_idem. vm_compute; auto.
-Qed.
-
-Lemma decode_int8_sign_ext:
-  forall l,
-  Int.sign_ext 31 8 (decode_int Mint8signed l) = decode_int Mint8signed l.
-Proof.
-  intros; simpl. apply Int.sign_ext_idem. vm_compute; auto.
-Qed.
-
-Lemma decode_int16_zero_ext:
-  forall l,
-  Int.zero_ext 31 16 (decode_int Mint16unsigned l) = decode_int Mint16unsigned l.
-Proof.
-  intros; simpl. apply Int.zero_ext_idem. vm_compute; auto.
-Qed.
-
-Lemma decode_int16_sign_ext:
-  forall l,
-  Int.sign_ext 31 16 (decode_int Mint16signed l) = decode_int Mint16signed l.
-Proof.
-  intros; simpl. apply Int.sign_ext_idem. vm_compute; auto.
-Qed.
-
-Lemma decode_int8_signed_unsigned:
-  forall l,
-  decode_int Mint8signed l = Int.sign_ext 31 8 (decode_int Mint8unsigned l).
-Proof.
-  intros; simpl. rewrite Int.sign_ext_zero_ext; auto. vm_compute; auto.
-Qed.
-
-Lemma decode_int16_signed_unsigned:
-  forall l,
-  decode_int Mint16signed l = Int.sign_ext 31 16 (decode_int Mint16unsigned l).
-Proof.
-  intros; simpl. rewrite Int.sign_ext_zero_ext; auto. vm_compute; auto.
+  intros. unfold encode_int. decEq.
+  unfold inj_int.
+  unfold wordsize_chunk in H. 
+  unfold bytesize_chunk in H.
+  apply bytes_of_int_mod' in H; try solve [apply ZRdiv_prop4].
+  rewrite H. auto.
 Qed.
 
 (** * Encoding and decoding floats *)
 
 Definition encode_float (c: memory_chunk) (f: float) : list byte :=
-  rev_if_be (match c with
-  | Mint8signed | Mint8unsigned => bytes_of_int 1%nat 0
-  | Mint16signed | Mint16unsigned => bytes_of_int 2%nat 0
-  | Mint32 => bytes_of_int 4%nat 0
+  rev_if_be _ (match c with
+  | Mint wz => bytes_of_int (bytesize_chunk_nat wz) 0
   | Mfloat32 => bytes_of_int 4%nat (Int.unsigned 31 (Float.bits_of_single f))
   | Mfloat64 => bytes_of_int 8%nat (Int.unsigned 63 (Float.bits_of_double f))
   end).
 
 Definition decode_float (c: memory_chunk) (b: list byte) : float :=
-  let b' := rev_if_be b in
+  let b' := rev_if_be _ b in
   match c with
   | Mfloat32 => Float.single_of_bits (Int.repr 31 (int_of_bytes b'))
   | Mfloat64 => Float.double_of_bits (Int.repr 63 (int_of_bytes b'))
@@ -395,7 +651,10 @@ Lemma encode_float_length:
 Proof.
   unfold encode_float; intros. 
   rewrite rev_if_be_length. 
-  destruct chunk; apply length_bytes_of_int. 
+  destruct chunk; try solve [
+    apply length_bytes_of_int |
+    unfold size_chunk_nat, size_chunk;
+      rewrite Z_of_nat_eq; apply length_bytes_of_int].
 Qed.
 
 Lemma decode_encode_float32: forall n,
@@ -423,18 +682,6 @@ Proof.
   rewrite Int.repr_unsigned. apply Float.double_of_bits_of_double.
 Qed.
 
-Lemma encode_float8_signed_unsigned: forall n,
-  encode_float Mint8signed n = encode_float Mint8unsigned n.
-Proof.
-  intros. reflexivity. 
-Qed.
-
-Lemma encode_float16_signed_unsigned: forall n,
-  encode_float Mint16signed n = encode_float Mint16unsigned n.
-Proof.
-  intros. reflexivity.
-Qed.
-
 Lemma encode_float32_cast:
   forall f,
   encode_float Mfloat32 (Float.singleoffloat f) = encode_float Mfloat32 f.
@@ -451,38 +698,6 @@ Proof.
 Qed.
 
 (** * Encoding and decoding values *)
-
-Definition inj_bytes (bl: list byte) : list memval :=
-  List.map Byte bl.
-
-Fixpoint proj_bytes (vl: list memval) : option (list byte) :=
-  match vl with
-  | nil => Some nil
-  | Byte b :: vl' =>
-      match proj_bytes vl' with None => None | Some bl => Some(b :: bl) end
-  | _ => None
-  end.
-
-Remark length_inj_bytes:
-  forall bl, length (inj_bytes bl) = length bl.
-Proof.
-  intros. apply List.map_length. 
-Qed.
-
-Remark proj_inj_bytes:
-  forall bl, proj_bytes (inj_bytes bl) = Some bl.
-Proof.
-  induction bl; simpl. auto. rewrite IHbl. auto.
-Qed.
-
-Lemma inj_proj_bytes:
-  forall cl bl, proj_bytes cl = Some bl -> cl = inj_bytes bl.
-Proof.
-  induction cl; simpl; intros. 
-  inv H; auto.
-  destruct a; try congruence. destruct (proj_bytes cl); inv H.
-  simpl. decEq. auto.
-Qed.
 
 Fixpoint inj_pointer (n: nat) (b: block) (ofs: Int.int 31) {struct n}: list memval :=
   match n with
@@ -502,53 +717,16 @@ Fixpoint check_pointer (n: nat) (b: block) (ofs: Int.int 31) (vl: list memval)
 Definition proj_pointer (vl: list memval) : val :=
   match vl with
   | Pointer b ofs n :: vl' =>
-      if check_pointer (size_chunk_nat Mint32) b ofs vl
+      if check_pointer (size_chunk_nat (Mint 31)) b ofs vl
       then Vptr b ofs
       else Vundef
   | _ => Vundef
   end.
 
-Definition encode_val (chunk: memory_chunk) (v: val) : list memval :=
-  match v, chunk with
-  | Vptr b ofs, Mint32 => inj_pointer (size_chunk_nat Mint32) b ofs
-  | Vint 31 n, _ => inj_bytes (encode_int chunk n)
-  | Vfloat f, _ => inj_bytes (encode_float chunk f)
-  | _, _ => list_repeat (size_chunk_nat chunk) Undef
-  end.
-
-Definition decode_val (chunk: memory_chunk) (vl: list memval) : val :=
-  match proj_bytes vl with
-  | Some bl =>
-      match chunk with
-      | Mint8signed | Mint8unsigned
-      | Mint16signed | Mint16unsigned | Mint32 =>
-          Vint 31 (decode_int chunk bl)
-      | Mfloat32 | Mfloat64 =>
-          Vfloat(decode_float chunk bl)
-      end
-  | None =>
-      match chunk with
-      | Mint32 => proj_pointer vl
-      | _ => Vundef
-      end
-  end.
-
-(*
 Lemma inj_pointer_length:
   forall b ofs n, List.length(inj_pointer n b ofs) = n.
 Proof.
   induction n; simpl; congruence.
-Qed.
-*)
-
-Lemma encode_val_length:
-  forall chunk v, length(encode_val chunk v) = size_chunk_nat chunk.
-Proof.
-  intros. destruct v; simpl.
-  apply length_list_repeat.
-  rewrite length_inj_bytes. apply encode_int_length.
-  rewrite length_inj_bytes. apply encode_float_length.
-  destruct chunk; try (apply length_list_repeat). reflexivity.
 Qed.
 
 Lemma check_inj_pointer:
@@ -559,27 +737,229 @@ Proof.
   rewrite <- beq_nat_refl. simpl; auto.
 Qed.
 
+Definition encode_val (chunk: memory_chunk) (v: val) : list memval :=
+  match v, chunk with
+  | Vptr b ofs, Mint wz => 
+    if eq_nat_dec wz 31 
+    then inj_pointer (size_chunk_nat (Mint wz)) b ofs
+    else list_repeat (size_chunk_nat chunk) Undef
+  | Vint wz n, Mint wz' =>
+    if eq_nat_dec wz wz' 
+    then encode_int wz n
+    else list_repeat (size_chunk_nat chunk) Undef
+  | Vfloat f, _ => inj_bytes (encode_float chunk f)
+  | _, _ => list_repeat (size_chunk_nat chunk) Undef
+  end.
+
+Definition decode_val (chunk: memory_chunk) (vl: list memval) : val :=
+  match chunk with
+  | Mint wz => 
+    match decode_int vl wz with
+    | Vundef => if eq_nat_dec wz 31 then proj_pointer vl else Vundef
+    | v => v
+    end
+  | Mfloat32 =>
+    match proj_bytes (bytesize_chunk_nat 31) vl with
+    | Some bl => Vfloat(decode_float chunk bl)
+    | None => Vundef
+    end
+  | Mfloat64 =>
+    match proj_bytes (bytesize_chunk_nat 63) vl with
+    | Some bl => Vfloat(decode_float chunk bl)
+    | None => Vundef
+    end
+  end.
+
+Lemma encode_val_length:
+  forall chunk v, length (encode_val chunk v) = size_chunk_nat chunk.
+Proof.
+  intros. destruct v; simpl.
+
+  apply length_list_repeat.
+
+  destruct chunk; simpl; unfold size_chunk_nat, size_chunk; auto with zarith.
+  destruct (eq_nat_dec wz n); subst.
+    apply encode_int_length.
+    apply length_list_repeat.
+
+  rewrite length_inj_bytes. apply encode_float_length.
+
+  destruct chunk; simpl; unfold size_chunk_nat, size_chunk; auto.
+    destruct (eq_nat_dec n 31); subst.
+      apply inj_pointer_length.
+      apply length_list_repeat.
+Qed.
+
 Definition decode_encode_val (v1: val) (chunk1 chunk2: memory_chunk) (v2: val) : Prop :=
   match v1, chunk1, chunk2 with
   | Vundef, _, _ => v2 = Vundef
-  | Vint n, Mint8signed, Mint8signed => v2 = Vint(Int.sign_ext 8 n)
-  | Vint n, Mint8unsigned, Mint8signed => v2 = Vint(Int.sign_ext 8 n)
-  | Vint n, Mint8signed, Mint8unsigned => v2 = Vint(Int.zero_ext 8 n)
-  | Vint n, Mint8unsigned, Mint8unsigned => v2 = Vint(Int.zero_ext 8 n)
-  | Vint n, Mint16signed, Mint16signed => v2 = Vint(Int.sign_ext 16 n)
-  | Vint n, Mint16unsigned, Mint16signed => v2 = Vint(Int.sign_ext 16 n)
-  | Vint n, Mint16signed, Mint16unsigned => v2 = Vint(Int.zero_ext 16 n)
-  | Vint n, Mint16unsigned, Mint16unsigned => v2 = Vint(Int.zero_ext 16 n)
-  | Vint n, Mint32, Mint32 => v2 = Vint n
-  | Vint n, Mint32, Mfloat32 => v2 = Vfloat(decode_float Mfloat32 (encode_int Mint32 n))
-  | Vint n, _, _ => True   (* nothing interesting to say about v2 *)
-  | Vptr b ofs, Mint32, Mint32 => v2 = Vptr b ofs
+
+  | Vint wz n, Mint wz1, Mint wz2 => 
+    if eq_nat_dec wz wz1
+    then 
+      if eq_nat_dec wz wz2
+      then v2 = Vint wz n
+      else v2 = Vundef
+    else v2 = Vundef
+  | Vint wz n, Mint wz', Mfloat32 => 
+    if eq_nat_dec wz 31
+    then 
+      if eq_nat_dec wz' 31
+      then 
+        match (proj_bytes (bytesize_chunk_nat wz) (encode_int wz n)) with
+        | Some bl => v2 = Vfloat(decode_float Mfloat32 bl)
+        | None => False
+        end
+      else True
+    else True
+  | Vint wz n, _, _ => True   (* nothing interesting to say about v2 *)
+
+  | Vptr b ofs, Mint wz1, Mint wz2 => 
+    if eq_nat_dec wz1 31
+    then 
+      if eq_nat_dec wz2 31
+      then v2 = Vptr b ofs
+      else v2 = Vundef
+    else v2 = Vundef
   | Vptr b ofs, _, _ => v2 = Vundef
+
   | Vfloat f, Mfloat32, Mfloat32 => v2 = Vfloat(Float.singleoffloat f)
-  | Vfloat f, Mfloat32, Mint32 => v2 = Vint(decode_int Mint32 (encode_float Mfloat32 f))
+  | Vfloat f, Mfloat32, Mint wz => 
+    if eq_nat_dec wz 31
+    then v2 = decode_int (inj_bytes (encode_float Mfloat32 f)) 31
+    else True
   | Vfloat f, Mfloat64, Mfloat64 => v2 = Vfloat f
   | Vfloat f, _, _ => True   (* nothing interesting to say about v2 *)
   end.
+
+Remark proj_bytes_undef:
+  forall n, (n > 0)%nat -> proj_bytes n (list_repeat n Undef) = None.
+Proof.
+  induction n; simpl; intro; auto.
+    contradict H; omega.
+Qed.
+
+Remark proj_pointer_undef:
+  forall n, proj_pointer (list_repeat n Undef) = Vundef.
+Proof.
+  induction n; simpl; auto.
+Qed.
+
+Lemma list_repeat_cons_inv : forall m a b,
+  a :: b = list_repeat m Undef ->
+  a = Undef /\
+  exists m', S m' = m /\ b = list_repeat m' Undef.
+Proof.
+  induction m; intros; simpl in *.
+    inversion H.
+
+    inversion H; subst.
+    split; auto.
+    exists m. split; auto.
+Qed.
+
+Lemma proj_int_undef : forall n m,
+  proj_int n (list_repeat m Undef) = None.
+Proof.
+  intros.
+  unfold proj_int.
+  remember (nat_of_Z (ZRdiv (Z_of_nat (S n)) 8)) as N.
+  induction N; simpl.
+    destruct (list_repeat m Undef); auto.
+
+    remember (list_repeat m Undef) as L.
+    destruct L; auto.
+      apply list_repeat_cons_inv in HeqL.
+      destruct HeqL as [H1 [m' [H2 H3]]]; subst; auto.
+Qed.      
+
+Lemma list_repeat_undef : forall n,
+  list_repeat n Undef ++ Undef :: nil =
+  Undef :: list_repeat n Undef.
+Proof.
+  induction n; simpl; auto.
+    rewrite IHn. auto.
+Qed.
+
+Lemma rev_if_be_nil : forall (A:Type), rev_if_be A nil = nil.
+Proof.
+  unfold rev_if_be.
+  destruct big_endian; auto.
+Qed.
+
+Lemma rev_if_be_repeat_undef : forall n,
+  rev_if_be _ (list_repeat n Undef) = list_repeat n Undef.
+Proof.
+  induction n; simpl.
+    apply rev_if_be_nil.
+
+    unfold rev_if_be in *.
+    destruct big_endian; auto.
+      simpl.
+      rewrite IHn. auto.
+      apply list_repeat_undef.
+Qed.
+
+Lemma proj_pointer_encode_int : forall wz i,
+  proj_pointer (encode_int wz i) = Vundef.
+Proof.
+  intros.
+  unfold proj_pointer, encode_int, inj_int.
+  destruct (bytes_of_int (nat_of_Z (ZRdiv (Z_of_nat (S wz)) 8)) (Int.unsigned wz i)); simpl; auto.
+    rewrite rev_if_be_nil. auto.
+Admitted.
+
+Lemma decode_int_repeat_Undef : forall n m,
+  decode_int (list_repeat n Undef) m = Vundef.
+Proof.
+  intros.
+  unfold decode_int.
+  rewrite rev_if_be_repeat_undef.
+  rewrite proj_int_undef. auto.
+Qed.
+
+Lemma proj_bytes_encode_int32 : forall i,
+  exists bl, proj_bytes (bytesize_chunk_nat 31) (encode_int 31 i) = Some bl.
+Admitted.
+
+Lemma decode_int_encode_float32 : forall f,
+  exists i, decode_int (inj_bytes (encode_float Mfloat32 f)) 31 = Vint 31 i.
+Admitted.
+
+Lemma proj_bytes_encode_float32 : forall f,
+  exists bl, proj_bytes (bytesize_chunk_nat 31) (inj_bytes (encode_float Mfloat32 f)) = Some bl.
+Admitted.      
+
+Lemma proj_bytes_encode_float64 : forall f,
+  exists bl, proj_bytes (bytesize_chunk_nat 63) (inj_bytes (encode_float Mfloat64 f)) = Some bl.
+Admitted.      
+
+Lemma encode_float32_length : forall f,
+  length (encode_float Mfloat32 f) = bytesize_chunk_nat 31.
+Admitted.
+
+Lemma encode_float64_length : forall f,
+  length (encode_float Mfloat64 f) = bytesize_chunk_nat 63.
+Admitted.
+
+Lemma decode_int_inj_pointer:
+  forall b ofs, 
+  decode_int (inj_pointer (size_chunk_nat (Mint 31)) b ofs) 31 = Vptr b ofs.
+Proof.
+Admitted.
+
+Lemma decode_int_inj_pointer_undef:
+  forall b ofs n, 
+  n <> 31%nat ->
+  decode_int (inj_pointer (size_chunk_nat (Mint 31)) b ofs) n = Vundef.
+Proof.
+Admitted.
+
+Remark proj_bytes_undef':
+  forall n m, (m > 0)%nat -> proj_bytes n (list_repeat m Undef) = None.
+Proof.
+  induction n; simpl; intros; auto.
+Admitted.
 
 Lemma decode_encode_val_general:
   forall v chunk1 chunk2,
@@ -590,70 +970,150 @@ Proof.
   simpl. destruct (size_chunk_nat_pos chunk1) as [psz EQ]. 
   rewrite EQ. simpl.
   unfold decode_val. simpl. destruct chunk2; auto.
+  change (Undef::list_repeat psz Undef) with (list_repeat (S psz) Undef).
+  rewrite decode_int_repeat_Undef.
+  destruct (eq_nat_dec n 31); subst; auto.
 (* Vint *)
   simpl.
-  destruct chunk1; auto; destruct chunk2; auto; unfold decode_val;
-  rewrite proj_inj_bytes.
-  rewrite decode_encode_int. auto.
-  rewrite encode_int8_signed_unsigned. rewrite decode_encode_int. auto.
-  rewrite <- encode_int8_signed_unsigned.  rewrite decode_encode_int. auto.
-  rewrite decode_encode_int. auto.
-  rewrite decode_encode_int. auto.
-  rewrite encode_int16_signed_unsigned. rewrite decode_encode_int. auto.
-  rewrite <- encode_int16_signed_unsigned.  rewrite decode_encode_int. auto.
-  rewrite decode_encode_int. auto.
-  rewrite decode_encode_int. auto.
-  reflexivity. 
+  destruct chunk1; auto; destruct chunk2; auto; unfold decode_val, encode_val; 
+  try rewrite proj_inj_bytes.
+
+    destruct (eq_nat_dec wz n); subst; auto.
+      destruct (eq_nat_dec n n0); subst; auto.
+        rewrite decode_encode_int_eq; auto.
+        rewrite decode_encode_int_neq; auto.
+        destruct (eq_nat_dec n0 31); subst; auto.
+          apply proj_pointer_encode_int.
+      rewrite decode_int_repeat_Undef.
+      destruct (eq_nat_dec n0 31); subst; auto.
+        apply proj_pointer_undef.
+      
+    destruct (eq_nat_dec wz 31); subst; auto.
+      destruct (eq_nat_dec n 31); subst; auto.
+        destruct (eq_nat_dec 31 31); subst.
+          destruct (@proj_bytes_encode_int32 i) as [bl EQ].
+          rewrite EQ.
+          simpl. auto.
+          
+          contradict n; auto.
 (* Vfloat *)
   unfold decode_val, encode_val, decode_encode_val;
-  destruct chunk1; auto; destruct chunk2; auto; unfold decode_val;
-  rewrite proj_inj_bytes.
-  auto.
-  rewrite decode_encode_float32. auto.
-  rewrite decode_encode_float64. auto.
+  destruct chunk1; auto; destruct chunk2; auto; unfold decode_val.
+
+    destruct (eq_nat_dec n 31); subst; auto.
+      destruct (@decode_int_encode_float32 f) as [i EQ].
+      rewrite EQ. auto.
+
+      destruct (@proj_bytes_encode_float32 f) as [bl EQ].
+      rewrite EQ. simpl.
+      decEq.
+      rewrite <- decode_encode_float32.
+      unfold decode_float.
+      rewrite <- (encode_float32_length f) in EQ.
+      rewrite proj_inj_bytes in EQ.
+      inversion EQ; subst; auto.
+
+    destruct (@proj_bytes_encode_float64 f) as [bl EQ].
+    rewrite EQ. simpl.
+    decEq.
+    rewrite <- decode_encode_float64.
+    unfold decode_float.
+    rewrite <- (encode_float64_length f) in EQ.
+    rewrite proj_inj_bytes in EQ.
+    inversion EQ; subst; auto.
+
 (* Vptr *)
   unfold decode_val, encode_val, decode_encode_val;
   destruct chunk1; auto; destruct chunk2; auto.
-  simpl. generalize (check_inj_pointer b i (size_chunk_nat Mint32)).
-  simpl. intro. rewrite H. auto.
+
+    destruct (eq_nat_dec n 31); subst; auto.
+      destruct (eq_nat_dec n0 31); subst; auto.
+        rewrite decode_int_inj_pointer; auto.
+        rewrite decode_int_inj_pointer_undef; auto.
+
+      rewrite decode_int_repeat_Undef.
+      destruct (eq_nat_dec n0 31); subst; auto.
+        rewrite proj_pointer_undef; auto.
+
+    destruct (eq_nat_dec n 31); subst; auto.
+      rewrite proj_bytes_undef'; auto using size_chunk_nat_pos'.
+
+    destruct (eq_nat_dec n 31); subst; auto.
+      rewrite proj_bytes_undef'; auto using size_chunk_nat_pos'.
+
+    rewrite decode_int_repeat_Undef.
+    destruct (eq_nat_dec n 31); subst; auto.
+   
+    rewrite decode_int_repeat_Undef.
+    destruct (eq_nat_dec n 31); subst; auto.
 Qed.
+
+Definition chunk_eq (c1 c2:memory_chunk) : Prop :=
+  size_chunk c1 = size_chunk c2 /\
+  match c1, c2 with
+  | Mint wz1, Mint wz2 => wz1 = wz2
+  | _, _ => True
+  end.
 
 Lemma decode_encode_val_similar:
   forall v1 chunk1 chunk2 v2,
   type_of_chunk chunk1 = type_of_chunk chunk2 ->
-  size_chunk chunk1 = size_chunk chunk2 ->
+  chunk_eq chunk1 chunk2 ->
   Val.has_type v1 (type_of_chunk chunk1) ->
   decode_encode_val v1 chunk1 chunk2 v2 ->
   v2 = Val.load_result chunk2 v1.
 Proof.
   intros. 
   destruct v1.
-  simpl in *. destruct chunk2; simpl; auto. 
+  simpl in *. destruct chunk2; simpl; auto.
+ 
   red in H1.
   destruct chunk1; simpl in H1; try contradiction;
   destruct chunk2; simpl in *; discriminate || auto.
+  destruct (eq_nat_dec wz n); subst.
+    destruct (eq_nat_dec n n0); subst.
+      destruct (eq_nat_dec n0 n0); subst; auto.
+        contradict n; auto.
+      destruct (eq_nat_dec n0 n); subst; auto.
+        contradict n1; auto.
+    destruct (eq_nat_dec n0 wz); subst; auto.
+      unfold chunk_eq in H0.
+      destruct H0; subst.
+      contradict n1; auto.
+
+  unfold chunk_eq in H0. destruct H0.
   red in H1.
   destruct chunk1; simpl in H1; try contradiction;
   destruct chunk2; simpl in *; discriminate || auto.
+    
+  unfold chunk_eq in H0. destruct H0.
   red in H1.
   destruct chunk1; simpl in H1; try contradiction;
   destruct chunk2; simpl in *; discriminate || auto.
+  subst.
+  destruct (eq_nat_dec n0 31); subst; auto.
 Qed.
 
 Lemma decode_val_type:
   forall chunk cl,
   Val.has_type (decode_val chunk cl) (type_of_chunk chunk).
 Proof.
-  intros. unfold decode_val. 
-  destruct (proj_bytes cl). 
+  intros. unfold decode_val.
   destruct chunk; simpl; auto. 
-  destruct chunk; simpl; auto.
-  unfold proj_pointer. destruct cl; try (exact I).
-  destruct m; try (exact I).
-  destruct (check_pointer (size_chunk_nat Mint32) b i (Pointer b i n :: cl));
-  exact I.
+
+    unfold decode_int.
+    destruct (proj_int n (rev_if_be memval cl)); simpl; auto.
+      destruct (eq_nat_dec n 31); simpl; auto.
+        unfold proj_pointer.
+        destruct cl; simpl; auto.
+          destruct m; simpl; auto.
+            destruct (check_pointer (size_chunk_nat (Mint 31)) b i (Pointer b i n0::cl)); simpl; auto.
+
+    destruct (proj_bytes (bytesize_chunk_nat 31) cl); simpl; auto.
+    destruct (proj_bytes (bytesize_chunk_nat 63) cl); simpl; auto.
 Qed.
 
+(*
 Lemma encode_val_int8_signed_unsigned:
   forall v, encode_val Mint8signed v = encode_val Mint8unsigned v.
 Proof.
@@ -689,53 +1149,77 @@ Lemma encode_val_int16_sign_ext:
 Proof.
   intros; unfold encode_val. rewrite encode_int16_sign_ext. auto.
 Qed.
+*)
 
 Lemma decode_val_int_inv:
-  forall chunk cl n,
-  decode_val chunk cl = Vint n ->
+  forall chunk cl n i,
+  decode_val chunk cl = Vint n i ->
   type_of_chunk chunk = Tint /\
-  exists bytes, proj_bytes cl = Some bytes /\ n = decode_int chunk bytes.
+  Vint n i = decode_int cl n.
 Proof.
-  intros until n. unfold decode_val. destruct (proj_bytes cl). 
-Opaque decode_int.
-  destruct chunk; intro EQ; inv EQ; split; auto; exists l; auto. 
-  destruct chunk; try congruence. unfold proj_pointer. 
-  destruct cl; try congruence. destruct m; try congruence. 
-  destruct (check_pointer (size_chunk_nat Mint32) b i (Pointer b i n0 :: cl));
-  congruence.
+  intros until i. unfold decode_val.
+  destruct chunk; intro EQ.
+    remember (decode_int cl n0) as R.
+    unfold decode_int in HeqR.
+    remember (proj_int n0 (rev_if_be memval cl)) as R'.
+    split. simpl. auto.
+      unfold decode_int.
+      destruct R'; subst.
+        inversion EQ; subst.
+        rewrite <- HeqR'. auto.
+
+        destruct (eq_nat_dec n0 31); subst; try solve [inversion EQ].
+          unfold proj_pointer in EQ.
+          destruct cl; try solve [inversion EQ].
+          destruct m; try solve [inversion EQ].
+          destruct (check_pointer (size_chunk_nat (Mint 31)) b i0 (Pointer b i0 n0::cl)); try solve [inversion EQ].
+
+    destruct (proj_bytes (bytesize_chunk_nat 31) cl); subst; try solve [inversion EQ].
+    destruct (proj_bytes (bytesize_chunk_nat 63) cl); subst; try solve [inversion EQ].
 Qed.
 
 Lemma decode_val_float_inv:
   forall chunk cl f,
   decode_val chunk cl = Vfloat f ->
   type_of_chunk chunk = Tfloat /\
-  exists bytes, proj_bytes cl = Some bytes /\ f = decode_float chunk bytes.
+  exists bl, proj_bytes (size_chunk_nat chunk) cl = Some bl /\ f = decode_float chunk bl.
 Proof.
-  intros until f. unfold decode_val. destruct (proj_bytes cl). 
-  destruct chunk; intro EQ; inv EQ; split; auto; exists l; auto. 
-  destruct chunk; try congruence. unfold proj_pointer. 
-  destruct cl; try congruence. destruct m; try congruence.
-  destruct (check_pointer (size_chunk_nat Mint32) b i (Pointer b i n :: cl));
-  congruence.
+  intros until f. unfold decode_val. 
+  destruct chunk; intro EQ.
+    remember (decode_int cl n) as R.
+    unfold decode_int in HeqR.
+    remember (proj_int n (rev_if_be memval cl)) as R'.
+    destruct R'; subst; try solve [inversion EQ].
+      destruct (eq_nat_dec n 31); subst; try solve [inversion EQ].
+        unfold proj_pointer in EQ.
+        destruct cl; try solve [inversion EQ].
+        destruct m; try solve [inversion EQ].
+        destruct (check_pointer (size_chunk_nat (Mint 31)) b i (Pointer b i n::cl)); try solve [inversion EQ].
+
+    remember (proj_bytes (bytesize_chunk_nat 31) cl) as R.
+    destruct R; subst; try solve [inversion EQ].
+    split; auto.
+      unfold decode_float in EQ.
+      inversion EQ; subst.
+      exists l. split; auto.
+
+    remember (proj_bytes (bytesize_chunk_nat 63) cl) as R.
+    destruct R; subst; try solve [inversion EQ].
+    split; auto.
+      unfold decode_float in EQ.
+      inversion EQ; subst.
+      exists l. split; auto.
 Qed.
 
 Lemma decode_val_cast:
   forall chunk l,
   let v := decode_val chunk l in
   match chunk with
-  | Mint8signed => v = Val.sign_ext 8 v
-  | Mint8unsigned => v = Val.zero_ext 8 v
-  | Mint16signed => v = Val.sign_ext 16 v
-  | Mint16unsigned => v = Val.zero_ext 16 v
   | Mfloat32 => v = Val.singleoffloat v
   | _ => True
   end.
 Proof.
-  unfold decode_val; intros; destruct chunk; auto; destruct (proj_bytes l); auto.
-  unfold Val.sign_ext. decEq. symmetry. apply decode_int8_sign_ext.
-  unfold Val.zero_ext. decEq. symmetry. apply decode_int8_zero_ext.
-  unfold Val.sign_ext. decEq. symmetry. apply decode_int16_sign_ext.
-  unfold Val.zero_ext. decEq. symmetry. apply decode_int16_zero_ext.
+  unfold decode_val; intros; destruct chunk; auto; destruct (proj_bytes (bytesize_chunk_nat 31) l); auto.
   unfold Val.singleoffloat. decEq. symmetry. apply decode_float32_cast. 
 Qed.
 
@@ -743,13 +1227,13 @@ Qed.
 
 Definition memval_valid_first (mv: memval) : Prop :=
   match mv with
-  | Pointer b ofs n => n = pred (size_chunk_nat Mint32)
+  | Pointer b ofs n => n = pred (size_chunk_nat (Mint 31))
   | _ => True
   end.
 
 Definition memval_valid_cont (mv: memval) : Prop :=
   match mv with
-  | Pointer b ofs n => n <> pred (size_chunk_nat Mint32)
+  | Pointer b ofs n => n <> pred (size_chunk_nat (Mint 31))
   | _ => True
   end.
 
@@ -774,11 +1258,25 @@ Proof.
     exploit list_in_map_inv; eauto. intros [x [A B]]. subst mv. exact I.
   destruct v; simpl. 
   auto.
+
+  destruct chunk; auto. 
+    destruct (eq_nat_dec wz n); subst; auto.
+      unfold encode_int.
+      admit. 
+
+  apply H0. apply encode_float_length.
+
+  destruct chunk; auto. 
+    destruct (eq_nat_dec n 31); subst; auto.
+      admit.
+(*
+  simpl; intros. intuition; subst mv; red; simpl; congruence.
   apply H0. apply encode_int_length. 
   apply H0. apply encode_float_length.
   destruct chunk; auto. 
   constructor. red. auto.
   simpl; intros. intuition; subst mv; red; simpl; congruence.
+*)
 Qed.
 
 Lemma check_pointer_inv:
@@ -810,7 +1308,11 @@ Lemma decode_val_shape:
   decode_val chunk mvl = Vundef \/ decoding_shape mvl.
 Proof.
   intros. destruct (size_chunk_nat_pos chunk) as [sz EQ]. 
-  unfold decode_val. 
+  unfold decode_val.
+  destruct chunk.
+    unfold decode_int.
+Admitted. 
+(*
   caseEq (proj_bytes mvl).
   intros bl PROJ. right. exploit inj_proj_bytes; eauto. intros. subst mvl.
   destruct bl; simpl in H. congruence. simpl. constructor. 
@@ -824,7 +1326,9 @@ Proof.
   constructor. red. auto. congruence. 
   simpl; intros. intuition; subst mv; simpl; congruence.
 Qed.
+*)
 
+(*
 Lemma encode_val_pointer_inv:
   forall chunk v b ofs n mvl,
   encode_val chunk v = Pointer b ofs n :: mvl ->
@@ -1056,5 +1560,6 @@ Lemma memval_inject_id:
   forall mv, memval_inject inject_id mv mv.
 Proof.
   destruct mv; econstructor. unfold inject_id; reflexivity. rewrite Int.add_zero; auto. 
-Qed.
- 
+Qed. 
+*)
+
